Estructura de ficheros

reduction_subsetSum_to_partition.dfy
@@ -1,14 +1,14 @@
-
-// Auxiliary functions
-
+// This function calculates the sum of the elements of a sequence
 function sum_seq(s:seq<int>): int
-	ensures |s| == 1 ==> sum_seq(s) == s[0]
+	ensures |s| == 1 ==> sum_seq(s) == s[0]  			
 {
 	if |s| == 0 then 0
 	else  s[0] + sum_seq(s[1..])
 }
 
 
+// This function creates a sequence from a multiset
+// This function will help later. 
 ghost function seq_from_multiset(ms:multiset<int>): seq<int>
 	ensures multiset(seq_from_multiset(ms)) == ms
 	
@@ -19,38 +19,36 @@ ghost function seq_from_multiset(ms:multiset<int>): seq<int>
 }
 
 
-ghost function sum_multiset(ms:multiset<int>): int
-{
-	var s := seq_from_multiset(ms);
-	sum_seq(s)
-}
-
-////////////////
-
-/**
-SubsetSum:
-SubsetSum is NP-Complete
- */
+// This problem is known as SubsetSum (it is NP-complete)
 ghost predicate subsetSum(t:int, r:seq<int>)
 {
 	exists s:seq<int>:: multiset(s) <= multiset(r) && sum_seq(s) == t
 }
 
 
-/**
-Partition:
- */
+// This problem is known as Partition.
 ghost predicate partition(r:seq<int>)
 {
 	exists s:seq<int>:: multiset(s) <= multiset(r)  && sum_seq(r) == 2*sum_seq(s)
 }
 
 
-//////////// SubsetSum reduces to Partition. Consequently Partition is NP-complete. 
-///////////  This is the proof of the reduction.
+/**
+The reduction: Subsetsum <=p Partition
+**/
 
+
+// Reduction function
+// The reduction only adds a new element to the sequence r.
+function subSetToPartition(t:int, r:seq<int>): seq<int>
+{
+	r + [sum_seq(r) - 2*t]
+}
+
+
+//Reduction correctness
 lemma reduction_Lemma  (t:int, r:seq<int>)
-	ensures subsetSum(t, r) <==> partition(r + [sum_seq(r) - 2*t]) 
+	ensures subsetSum(t, r) <==> partition(subSetToPartition(t, r)) 
 {
 	if subsetSum(t, r) 
 	{
@@ -65,16 +63,16 @@ lemma reduction_Lemma  (t:int, r:seq<int>)
 
 lemma reduction_Lemma_right (t:int, r:seq<int>)
 	requires subsetSum(t, r) 
-	ensures partition(r + [sum_seq(r) - 2*t]) 
+	ensures partition(subSetToPartition(t, r)) 
 
 {
 	forall_distributive_sum_seq_Lemma();
-	var nr := r + [sum_seq(r) - 2*t];
+	//var nr := r + [sum_seq(r) - 2*t];
 	var s :|  multiset(s) <= multiset(r) && sum_seq(s) == t;
 	var ns := s + [sum_seq(r) - 2*t]; 
-	assert sum_seq(ns) == sum_seq(r) - t;
-	assert  multiset(ns) <= multiset(nr)  && sum_seq(nr) == 2*sum_seq(ns);
-	assert partition(nr);	
+	//assert sum_seq(ns) == sum_seq(r) - t;
+	//assert  multiset(ns) <= multiset(nr)  && sum_seq(nr) == 2*sum_seq(ns);
+	//assert partition(nr);	
 }
 
 
@@ -87,37 +85,18 @@ lemma reduction_Lemma_left (t:int, r:seq<int>)
 	var i := sum_seq(r) - 2*t;
 	var nr := r + [i];
 	var s :| multiset(s) <= multiset(nr)  && sum_seq(nr) == 2*sum_seq(s);	
-	assert sum_seq(s) == sum_seq(r) - t;
+	//assert sum_seq(s) == sum_seq(r) - t;
 	if i !in multiset(s)
 	{
 		var sm := seq_from_multiset(multiset(r) - multiset(s));
-		same_sum_Lemma(sm + s, r);									//Same multisets have the same sum.
-		
-		calc ==
-		{	
-			sum_seq(r);
-			sum_seq(sm + s);
-			sum_seq(sm) + sum_seq(s);
-		}
-		assert sum_seq(sm) == t;  		
-		assert multiset(sm) <= multiset(r) && sum_seq(sm) == t;		//Def. of subsetSum.
-		assert subsetSum(t, r);
+		same_sum_Lemma(sm + s, r); //Same multisets have the same sum.
 	}
 	else
 	{
 		
 		var sm := seq_from_multiset(multiset(s) - multiset{i}); 
-		same_sum_Lemma(sm + [i], s);							//Same multisets have the same sum.
-		calc ==
-		{
-			sum_seq(s);
-			sum_seq(sm + [i]);
-			sum_seq(sm) + i;
-		}
-		assert sum_seq(sm) == t;  		
-		assert multiset(sm) <= multiset(r) && sum_seq(sm) == t;	//Def. of subsetSum.
+		same_sum_Lemma(sm + [i], s); //Same multisets have the same sum.
 		
-		assert subsetSum(t, r);
 	}
 }
 
@@ -159,13 +138,15 @@ lemma same_sum_Lemma(s:seq<int>, r:seq<int>)
 		//assert r[0] in s;
 		var j :| 0 <= j < |s| && s[j] == r[0];
 		assert s == s[..j] + [r[0]] + s[j+1..];
-		assert sum_seq(s) == sum_seq(s[..j]) + r[0] + sum_seq(s[j+1..]);//sum_seq  distributes.
+		//assert sum_seq(s) == sum_seq(s[..j]) + r[0] + sum_seq(s[j+1..]); //sum_seq  distributes.
 		var ss := s[..j] + s[j+1..];								
-		assert sum_seq(ss) == sum_seq(s[..j]) + sum_seq(s[j+1..]); 		//sum_seq distributes.
+		//assert sum_seq(ss) == sum_seq(s[..j]) + sum_seq(s[j+1..]); //sum_seq distributes.
 		assert multiset(ss) == multiset(s) - multiset{r[0]};
-		same_sum_Lemma(ss, r[1..]);										//Same multisets have the same sum.				
-		assert sum_seq(r[1..]) == sum_seq(ss);							//H.I.				
-		assert r[0] + sum_seq(r[1..]) == r[0] + sum_seq(ss); 			//Def. sum_seq.
-		assert sum_seq(r) == sum_seq(s);
+		same_sum_Lemma(ss, r[1..]);	//Same multisets have the same sum.				
+		//assert sum_seq(r[1..]) == sum_seq(ss); //H.I.				
+		//assert r[0] + sum_seq(r[1..]) == r[0] + sum_seq(ss); 	//Def. sum_seq.
+		//assert sum_seq(r) == sum_seq(s);
 	}
 }
+
+
