reduction_clique_to_independentSet.dfy
@@ -1,0 +1,97 @@
+datatype Graph = G(V: nat, E: set<(nat, nat)>)
+// Note: The nodes of the graph are natural numbers from 1 to |V|
+// The edges (u, v) in E always satisfy that u < v
+
+
+// This predicate guarantees that the nodes of the edges are nodes of the graph
+ghost predicate valid_graph(g: Graph)
+{
+    forall u, v :: (u, v) in g.E ==> 0 < u < v <= g.V
+}
+
+
+// This predicate is the decision problem known as the Clique problem
+ghost predicate clique(g: Graph, k: nat)
+    requires valid_graph(g)
+{
+    exists cl: set<nat> :: |cl| == k && 
+    (
+        forall u, v :: 0 < u < v <= g.V ==> u in cl && v in cl ==> (u, v) in g.E 
+    )
+}
+
+
+// This predicate is the decision problem known as the Independent-Set problem
+ghost predicate independentSet(g: Graph, k: nat)
+    requires valid_graph(g)
+{
+    exists ins: set<nat> :: |ins| == k && 
+    (
+        forall u, v :: 0 < u < v <= g.V ==> u in ins && v in ins ==> (u, v) !in g.E 
+    )
+}
+
+
+/**
+The reduction: Clique <=p Independent-Set
+**/
+
+
+// Reduction function
+
+// This function calculates the complementary set of edges
+function complementary_edges(g: Graph): set<(nat, nat)>
+    requires valid_graph(g)
+    ensures forall u, v:: (u, v) in complementary_edges(g) ==> 0 < u < v <= g.V
+    ensures forall u, v :: 0 < u < v <= g.V ==> 
+        (
+            (u, v) in g.E <==> (u, v) !in complementary_edges(g)
+        )
+{
+   
+    set u, v | 0 < u < v <= g.V && (u,v) !in g.E :: (u, v)    
+} 
+
+
+// The reduction function only transforms the initial graph G(V,E) into G(V,E')
+// where E' is the complementary set of E  
+function inverse_graph(g: Graph): Graph
+    requires valid_graph(g)
+    ensures valid_graph(inverse_graph(g))
+    ensures g.V == inverse_graph(g).V
+    ensures forall u, v :: 0 < u < v <= g.V ==> 
+        (
+            (u, v) in g.E <==> (u, v) !in inverse_graph(g).E
+        )
+{
+    if g.V == 0 then g else G(g.V, complementary_edges(g))
+}
+
+
+//Reduction correctness
+lemma reduction_Lemma(g: Graph, k: nat)
+    requires valid_graph(g)
+    ensures clique(g, k) <==> independentSet(inverse_graph(g), k)
+{
+    if clique(g, k)
+    {
+        reduction_Lemma_right(g, k);
+    }
+    if independentSet(inverse_graph(g), k)
+    {
+        reduction_Lemma_left(g, k);
+    }
+}
+
+lemma reduction_Lemma_right(g: Graph, k: nat)
+    requires valid_graph(g)
+    requires clique(g, k)
+    ensures independentSet(inverse_graph(g), k)
+{}
+
+lemma reduction_Lemma_left(g: Graph, k: nat)
+    requires valid_graph(g)
+    requires independentSet(inverse_graph(g), k)
+    ensures clique(g, k)
+{}
+
