reduction_independentSet_to_vertexCover.dfy
@@ -1,0 +1,72 @@
+datatype Graph = G(V: set<nat>, E: set<(nat, nat)>)
+// The nodes of the graph are natural numbers
+
+// The nodes of the edge are nodes of the graph and every edge (u, v) always satisfy u<v
+ghost predicate validGraph(g: Graph)
+{
+    forall e :: e in g.E ==> (e.0 in g.V && e.1 in g.V) && e.0 < e.1
+}
+
+// This predicate is the decision problem known as the Independent-Set problem
+ghost predicate independentSet(g: Graph, k: nat)
+    requires validGraph(g)
+{
+    exists ins: set<nat> :: |ins| == k && ins<=g.V &&
+    (
+        forall u, v :: u in g.V && v in g.V && u!=v ==> u in ins && v in ins ==> (u, v) !in g.E
+    )
+}
+
+// This predicate is true if 'ins' is an independent set of size 'k' in the graph 'g'
+ghost predicate is_independentSet(g: Graph, k: nat, ins: set<nat>)
+    requires validGraph(g)
+    ensures is_independentSet(g, k, ins) ==> independentSet(g, k)
+{
+    |ins| == k && ins<=g.V && (forall u, v :: u in g.V && v in g.V && u!=v ==> u in ins && v in ins ==> (u, v) !in g.E)
+}
+
+// This predicate is the decision problem known as the Vertex-Cover problem
+ghost predicate vertexCover(g: Graph, k: nat)
+    requires validGraph(g)
+{
+    exists vc: set<nat> :: |vc| == k && vc<=g.V &&
+    (
+        forall e :: e in g.E ==> (e.0 in vc || e.1 in vc)
+    )
+}
+
+// This predicate is true if 'vc' is a vertex cover of size 'k' in the graph 'g'
+ghost predicate is_vertexCover(g: Graph, k: nat, vc: set<nat>)
+    requires validGraph(g)
+    ensures is_vertexCover(g, k, vc) ==> vertexCover(g, k)
+{
+    |vc| == k && vc<=g.V && (forall e :: e in g.E ==> (e.0 in vc || e.1 in vc))
+}
+
+/**
+The reduction: independentSet <=p vertexCover
+ */
+
+// Reduction correctness
+lemma independentSet_to_vertexCover_Lemma(g: Graph, k: nat)
+    requires validGraph(g)
+    requires |g.V| >= k //
+    ensures independentSet(g, k) <==> vertexCover(g, |g.V|-k)
+{
+    if independentSet(g, k)
+    {
+        var ins: set<nat> :| is_independentSet(g, k, ins);
+        independentSet_to_vertexCover_sub_Lemma(g, k, ins);
+    }
+    if vertexCover(g, |g.V|-k)
+    {
+        var ins: set<nat> :| is_vertexCover(g, |g.V|-k, g.V-ins);
+    }
+}
+
+lemma independentSet_to_vertexCover_sub_Lemma(g: Graph, k: nat, ins: set<nat>)
+    requires validGraph(g)
+    requires |g.V| >= k //sino dafny se queja en la llamada del ensures
+    requires ins <= g.V //hasta qué punto es trampa?
+    ensures is_independentSet(g, k, ins) <==> is_vertexCover(g, |g.V|-k, g.V-ins)
+{}
